Phi_Examples/Dynamic_Array.thy
@@ -67,6 +67,7 @@ proc Max:
   if (x < y) \<medium_left_bracket> y \<medium_right_bracket> \<medium_left_bracket> x \<medium_right_bracket>
 \<medium_right_bracket> .
 
+
 proc push_dynarr:
   input    \<open>l \<Ztypecolon> \<r>\<e>\<f> DynArr addr T\<heavy_comma> v \<Ztypecolon> \<v>\<a>\<l> T\<close>
   premises \<open>length l \<le> 2^(addrspace_bits-2) \<and> 2 \<le> addrspace_bits\<close>
