Phi_Semantics/PhiSem_Machine_Integer_Boolean.thy
@@ -2,13 +2,17 @@ theory PhiSem_Machine_Integer_Boolean
   imports PhiSem_Machine_Integer
 begin
 
-specification (bool) bool_def'[discharging_semantic_debt]:
-  \<open>bool = int(1)\<close> by blast
+specification (\<b>\<o>\<o>\<l>)
+  bool_def'[discharging_semantic_debt]: \<open>\<b>\<o>\<o>\<l> = int(1)\<close> by blast
 
-specification (V_bool) V_bool_def'[discharging_semantic_debt]:
-    \<open>V_bool = Virtual_Datatype.lift_Field (\<lambda>(_,x). x = 1) (\<lambda>b. (1, if b then 1 else 0)) V_int\<close>
-  by blast
+specification (sem_mk_bool)
+  sem_mk_bool_def'[discharging_semantic_debt]: \<open>sem_mk_bool b = sem_mk_int (1, if b then 1 else 0)\<close>
+  by fastforce
 
-hide_fact bool_def V_bool_def
+specification (sem_dest_bool)
+  sem_dest_bool'[discharging_semantic_debt]:
+    \<open>sem_dest_bool v = (snd (sem_dest_int v) = 1)\<close>
+  by fastforce
+
 
 end
